theories/logrel/F_mu/soundness.v
@@ -10,7 +10,7 @@ Proof.
   intros Hlog ??. cut (adequate NotStuck e σ (λ _ _, True)); first (intros [_ ?]; eauto).
   eapply (wp_adequacy Σ); eauto.
   iIntros (Hinv ?). iModIntro. iExists (λ _ _, True%I). iSplit=> //.
-  rewrite -(empty_env_subst e).
+  replace e with e.[env_subst[]] by by asimpl.
   set (HΣ := IrisG _ _ Hinv (λ _ _ _, True)%I (λ _, True)%I).
   iApply (wp_wand with "[]"). iApply Hlog; eauto. by iApply interp_env_nil. auto.
 Qed.
